compiler/src/compiler/RecurseWithFun.v
@@ -1,0 +1,54 @@
+(*almost copied verbatim from the standard library*)
+(*allows for general recursion where one argument to recursive function is a function, without using funext axiom *)
+Section FixPoint.
+
+Variable A : Type.
+Variable R : A -> A -> Prop.
+Hypothesis Rwf : well_founded R.
+Variable P : Type. (* really I want to say that P gives one type for each equivalence class
+                      of A wrt the equivalence relation E.  Not clear how to say this though.*)
+Variable F : forall x:A, (forall y:A, R y x -> P) -> P.
+Variable E : A -> A -> Prop.
+
+Fixpoint my_Fix_F (x:A) (a:Acc R x) : P :=
+  F x (fun (y:A) (h:R y x) => my_Fix_F y (Acc_inv a h)).
+
+Scheme Acc_inv_dep := Induction for Acc Sort Prop.
+
+Lemma my_Fix_F_eq (x:A) (r:Acc R x) :
+  F x (fun (y:A) (p:R y x) => my_Fix_F y (Acc_inv r p)) = my_Fix_F x r.
+Proof.
+  destruct r using Acc_inv_dep; auto.
+Qed.
+
+Definition my_Fix (x:A) := my_Fix_F x (Rwf x).
+
+(** Proof that [well_founded_induction] satisfies the fixpoint equation.
+    It requires an extra property of the functional *)
+
+Hypothesis
+  F_ext :
+  forall (x1 x2:A) (f1:forall y:A, R y x1 -> P) (f2:forall y:A, R y x2 -> P),
+    E x1 x2 ->
+    (forall (y1 y2:A) (p1:R y1 x1) (p2:R y2 x2),
+        E y1 y2 -> f1 y1 p1 = f2 y2 p2) -> F x1 f1 = F x2 f2.
+
+Lemma my_Fix_F_inv : forall (x1 x2:A) (r1:Acc R x1) (r2:Acc R x2),
+    E x1 x2 -> my_Fix_F x1 r1 = my_Fix_F x2 r2.
+Proof.
+  intro x1; induction (Rwf x1); intros x2 r1 r2.
+  rewrite <- (my_Fix_F_eq x r1); rewrite <- (my_Fix_F_eq x2 r2); intros.
+  apply F_ext; auto.
+Qed.
+
+Lemma my_Fix_eq : forall (x1 x2:A),
+    E x1 x2 -> my_Fix x1 = F x2 (fun (y:A) (p:R y x2) => my_Fix y).
+Proof.
+  intro x; unfold my_Fix.
+  rewrite <- my_Fix_F_eq.
+  intros. apply F_ext; intros.
+  - assumption.
+  - apply my_Fix_F_inv. assumption.
+Qed.
+
+End FixPoint.
